before giving up on multiple encoded values

HouLean/Meta/SpecializeAndSimp2/Encoding.lean
@@ -31,21 +31,109 @@ theorem uncurry_eval_succ (f : X → F) (xs) : uncurry f xs = uncurry (f xs.1) x
 
 end Uncurry
 
-class TypeEncoding (F : outParam (Type u)) {Xs : outParam (Type v)} {Y : Type u} [Uncurry F Xs Y] where
-  encode : Y → Xs
-  decode : F
-  valid : uncurry decode ∘ encode = id
 
+class TypeEncoding (X : Type) (Y : outParam Type) where
+  encode : X → Y
+  decode : Y → X
+  decode_encode : ∀ x, decode (encode x) = x
 
-variable {X' Y'} [TypeEncoding (X' → Y')]
-variable {F Xs Y} [Uncurry F Xs Y] [TypeEncoding F]
+attribute [simp] TypeEncoding.decode_encode
 
 open TypeEncoding
 
-@[simp]
-theorem decode_encode (y : Y) : (uncurry (decode (Y:=Y))) (encode y) = y :=
-  congrFun TypeEncoding.valid y
+instance [TypeEncoding X Y] [TypeEncoding X' Y'] : TypeEncoding (X×X') (Y×Y') where
+  encode x := (encode x.1, encode x.2)
+  decode x := (decode x.1, decode x.2)
+  decode_encode := by simp
 
-@[simp]
-theorem decode_encode' (y : Y') : decode (Y:=Y') (encode y) = y :=
-  decode_encode y
+instance : TypeEncoding Float Float where
+  encode x := x
+  decode x := x
+  decode_encode := by simp
+
+instance : TypeEncoding Float32 Float32 where
+  encode x := x
+  decode x := x
+  decode_encode := by simp
+
+instance : TypeEncoding Nat Nat where
+  encode x := x
+  decode x := x
+  decode_encode := by simp
+
+instance : TypeEncoding Int Int where
+  encode x := x
+  decode x := x
+  decode_encode := by simp
+
+instance : TypeEncoding UInt64 UInt64 where
+  encode x := x
+  decode x := x
+  decode_encode := by simp
+
+instance : TypeEncoding UInt32 UInt32 where
+  encode x := x
+  decode x := x
+  decode_encode := by simp
+
+instance : TypeEncoding UInt16 UInt16 where
+  encode x := x
+  decode x := x
+  decode_encode := by simp
+
+instance : TypeEncoding Int64 Int64 where
+  encode x := x
+  decode x := x
+  decode_encode := by simp
+
+instance : TypeEncoding Int32 Int32 where
+  encode x := x
+  decode x := x
+  decode_encode := by simp
+
+instance : TypeEncoding Int16 Int16 where
+  encode x := x
+  decode x := x
+  decode_encode := by simp
+
+@[simp] theorem Int.encode (x : Int) : encode x = x := by rfl
+@[simp] theorem Int.decode (x : Int) : decode x = x := by rfl
+@[simp] theorem Nat.encode (x : Nat) : encode x = x := by rfl
+@[simp] theorem Nat.decode (x : Nat) : decode x = x := by rfl
+
+instance [TypeEncoding X Y] [Inhabited X] : TypeEncoding (Option X) (Y × Bool) where
+  encode x? := (encode (x?.getD default), x?.isSome)
+  decode := fun (value, valid) => if valid then some (decode value) else none
+  decode_encode := by intro x; cases x <;> simp
+
+structure Vector2 (X : Type) where
+  (x0 x1 : X)
+
+instance [TypeEncoding X Y] : TypeEncoding (Vector X 2) (Vector2 Y) where
+  encode u := { x0 := encode u[0], x1 := encode u[1] }
+  decode u := #v[decode u.x0, decode u.x1 ]
+  decode_encode := sorry_proof
+
+structure Vector3 (X : Type) where
+  (x0 x1 x2 : X)
+
+instance [TypeEncoding X Y] : TypeEncoding (Vector X 3) (Vector3 Y) where
+  encode u := { x0 := encode u[0], x1 := encode u[1], x2 := encode u[2] }
+  decode u := #v[decode u.x0, decode u.x1, decode u.x2]
+  decode_encode := sorry_proof
+
+variable {X Y} [TypeEncoding X Y]
+@[simp] theorem Vector3.decode_getElem_0 (u : Vector3 Y) : (decode (X:=Vector X 3) u)[0] = decode u.x0 := by rfl
+@[simp] theorem Vector3.decode_getElem_1 (u : Vector3 Y) : (decode (X:=Vector X 3) u)[1] = decode u.x1 := by rfl
+@[simp] theorem Vector3.decode_getElem_2 (u : Vector3 Y) : (decode (X:=Vector X 3) u)[2] = decode u.x2 := by rfl
+@[simp] theorem Vector3.encode_vector_mk (x y z : X) : encode #v[x,y,z] = ⟨encode x, encode y, encode z⟩ := by rfl
+
+structure Vector4 (X : Type) where
+  (x0 x1 x2 x3 : X)
+
+instance [TypeEncoding X Y] : TypeEncoding (Vector X 4) (Vector4 Y) where
+  encode u := { x0 := encode u[0], x1 := encode u[1], x2 := encode u[2], x3 := encode u[3] }
+  decode u := #v[decode u.x0, decode u.x1, decode u.x2, decode u.x3]
+  decode_encode := sorry_proof
+
+-- #check (by infer_instance : TypeEncoding (Vector (Vector Float 3) 2) _)
