HouLean/Meta/SpecializeAndSimp2/Encoding/Option.lean
@@ -13,14 +13,54 @@ namespace Option
 @[simp] theorem decode_true (x : α) : Option.decode x true = some x := by simp [Option.decode]
 @[simp] theorem decode_false (x : α) : Option.decode x false = none := by simp [Option.decode]
 
-@[simp] theorem decode_getD (x y : α) (valid : Bool) :
-    (Option.decode x valid).getD y = if valid then x else y := by
-  cases valid <;> simp [Option.decode]
+-- @[simp] theorem decode_getD (x y : α) (valid : Bool) :
+--     (Option.decode x valid).getD y = if valid then x else y := by
+--   cases valid <;> simp [Option.decode]
 
-@[simp] theorem decode_isSome (x : α) (valid : Bool) :
-    (Option.decode x valid).isSome = valid := by
-  cases valid <;> simp [Option.decode]
+-- @[simp] theorem decode_isSome (x : α) (valid : Bool) :
+--     (Option.decode x valid).isSome = valid := by
+--   cases valid <;> simp [Option.decode]
 
-@[simp] theorem decode_isNone (x : α) (valid : Bool) :
-    (Option.decode x valid).isNone = !valid := by
-  cases valid <;> simp [Option.decode]
+-- @[simp] theorem decode_isNone (x : α) (valid : Bool) :
+--     (Option.decode x valid).isNone = !valid := by
+--   cases valid <;> simp [Option.decode]
+
+
+def encodeVal {α} [Inhabited α] (x : Option α) : α := x.getD default
+def encodeValid {α} [Inhabited α] (x : Option α) : Bool := x.isSome
+
+@[simp]
+theorem encodeVal_some {α} [Inhabited α] (x : α) : encodeVal (some x) = x := by simp[encodeVal]
+@[simp]
+theorem encodeVal_none {α} [Inhabited α] : encodeVal (none : Option α) = default := by simp[encodeVal]
+
+@[simp]
+theorem encodeValid_some {α} [Inhabited α] (x : α) : encodeValid (some x) = true := by simp[encodeValid]
+@[simp]
+theorem encodeValid_none {α} [Inhabited α] : encodeValid (none : Option α) = false := by simp[encodeValid]
+
+
+-- all these are getting out of hand, ... how to connect them to the actual Option API?
+@[simp]
+theorem decode_encode {α} [Inhabited α] (x : Option α) :
+  decode x.encodeVal x.encodeValid = x := by cases x <;> simp
+
+@[simp]
+theorem encodeValid_decode {α} [Inhabited α] (x : α) (v : Bool) :
+  encodeValid (decode x v) = v := by cases v <;> simp
+
+@[simp]
+theorem encodeVal_decode {α} [Inhabited α] (x : α) (v : Bool) :
+  encodeVal (decode x v) = if v then x else default := by cases v <;> simp
+
+@[simp]
+theorem decode_ite {α} [Inhabited α] (x y : α) (v : Bool) :
+  decode (if v then x else y) v = decode x v := by cases v <;> simp
+
+-- @[simp]
+-- theorem encodeVal_decode {α} [Inhabited α] (x : α) (v : Bool) :
+--   encodeVal (decode x v) = if v then x else  := by cases v <;> simp
+
+
+
+theorem decode_if {α} [Inhabited α] (x : α) (valid : Bool) : Option.decode (if valid then x else default) valid = Option.decode x valid := by cases valid <;> simp[Option.decode]
