HouLean/Meta/SpecializeAndSimp2/Command.lean
@@ -8,6 +8,11 @@ elab "#sas " e:term : command =>
   withoutModifyingEnv do
   runTermElabM fun _ctx => do
     let e ← elabTermAndSynthesize e none
-    let e ← sas e #[`simp]
-    logInfo e
-    pure ()
+    let (e,specs) ← sas e #[`simp]
+
+    let mut m : MessageData := m!""
+    for s in specs.reverse do
+      let info ← getConstInfo s.implName
+      m := m ++ m!"def {s.req.specName} := {indentExpr info.value!}\n\n"
+    m := m ++ m!"{e}"
+    logInfo m
