Tests/Meta/SpecAndSimp.lean
@@ -1,14 +1,185 @@
-import HouLean.Meta.SpecializeAndSimp.Main
-import HouLean.OpenCL.Basic
--- import HouLean.OpenCL.Data.Fin
-import HouLean.OpenCL.Data.InlinedLoop
-import HouLean.OpenCL.Reference.Operators
-import HouLean.Data.Matrix
+import HouLean.Meta.SpecializeAndSimp2.Main
+import HouLean.Meta.SpecializeAndSimp2.Command
+import HouLean.Meta.FloatPolynomial
 import HouLean.Data.Vector
--- import HouLean.OpenCL.Data.Matrix
+import HouLean.Meta.RewriteBy
 
-import Qq
+namespace Test.Meta.Sas2
 
-open Lean Meta Qq HouLean Meta
+open Lean Elab Command Term
 
-namespace Test.OpenCL.SpecAndSimp
+open HouLean.Meta.Sas
+
+
+-- set_option trace.HouLean.sas true
+-- set_option trace.HouLean.sas.simp true
+
+simproc ↓ binder_backstop (_) := fun e => do
+  if e.isLambda ||
+     e.isLet ||
+     (← Meta.isMatcherApp e) then
+    return .done { expr := e }
+  return .continue
+
+#sas fun x y : Nat =>
+  let a :=
+    let a1 := x + 0 + y
+    let a2 := 1 * a1 * 1 * x * 1
+    a1 + a2 + x
+  let b := x * y
+  a + b + y
+
+#sas fun x : Float => x + 0
+
+@[simp]
+theorem add_self (x : Nat) : x + x = 2 * x := by grind
+
+#sas fun x : Nat =>
+  let a := x*x + 0
+  a + x
+
+def id' {α} (a : α) := a
+
+#sas fun x : Nat =>
+  let a := some x
+  let a := a.map (·+1)
+  a.getD 0 + x
+
+def f1 {α} [Inhabited α] (x : Option α) := x.getD default
+
+#sas fun x : Option Float => f1 x
+
+set_option pp.funBinderTypes true
+
+/-- info: fun (x : VectorFloat3) => x -/
+#guard_msgs in
+#sas fun x : Vector Float 3 => x
+
+/-- info: fun (x : VectorFloat3) => x.x0 -/
+#guard_msgs in
+#sas fun x : Vector Float 3 => x[0]
+
+/-- info: fun (x : VectorFloat3) => x.x1 -/
+#guard_msgs in
+#sas fun x : Vector Float 3 => x[1]
+
+/-- info: fun (x : VectorFloat3) => x.x2 -/
+#guard_msgs in
+#sas fun x : Vector Float 3 => x[2]
+
+def f2 {α : Type} (x : Vector α 3) := x
+
+#sas fun x y z : Float => #v[x,y,z]
+
+/--
+info: fun (x : VectorFloat3) =>
+  let tmp := Neg.neg.Vector_Float_3 x;
+  tmp
+-/
+#guard_msgs in
+#sas fun x : Vector Float 3 => - x
+
+def addVectors {α n} [Add α] (x y : Vector α n) (bias? : Option α) :=
+  if let some bias := bias? then
+    (x + y).map (·+bias)
+  else
+    (x + y)
+
+
+def integrateParticle {α n} [One α] [Sub α] [Add α] [Mul α]
+    (x v : Vector α n) (dt : α)
+    (force? : Option (Vector α n)) (drag? : Option α) :
+    Vector α n × Vector α n := Id.run do
+  let mut x := x
+  let mut v := v
+  if let some f := force? then
+    v := v + dt * f
+  if let some drag := drag? then
+    v := (1 - dt * drag) * v
+  x := x + dt * v
+  return (x,v)
+
+#print integrateParticle
+
+def foo {α n} (x : Vector α n) : Option (Vector α n) := some x
+
+def bar {α} (x : α) : Option α := some x
+
+-- set_option pp.funBinderTypes true
+
+#check Vector.zipWith
+#check VectorFloat3.fromVector
+
+set_option trace.HouLean.sas true
+
+#sas fun (x y : VectorFloat3) => -x.toVector
+
+-- #sas fun (x y : Vector Float 3) (a : Float) =>
+--   addVectors x y (some a)
+
+-- #sas fun (x v f : Vector Float 3) (d : Float) =>
+--   integrateParticle x (addVectors v v (some 2)) 0.1 (foo f) (bar d)
+
+#sas fun (x : Vector Float 3) =>
+  if x[0] + x[1] > 0 then
+    some (x[0] + x[1] + x[2])
+  else
+    none
+
+#check @ite
+
+set_option trace.HouLean.sas true in
+set_option trace.HouLean.sas.simp true in
+#sas fun (x : Vector Float 3) => x[0] + x[1]
+
+
+structure Particle (X : Type) where
+  position : X
+  velocity : X
+
+def system [Add X] [HMul R X X] [Zero X]
+    (force? : Option (X → X)) (drag? : Option R) (x v : X) : X × X := Id.run do
+  let mut force : X := 0
+  if let some f := force? then
+    force := force + f x
+  if let some drag := drag? then
+    force := force + drag * v
+  return (v, force)
+
+def bar' (x : Float) (a? b? : Option Float) := Id.run do
+  let mut x := x
+  if let some a := a? then
+    x := x + a
+  if let some b := b? then
+    x := x + b
+  return x
+
+#print bar'
+
+variable (x a : Float) (b? : Option Float)
+
+@[simp]
+theorem bind_id (x : Id α) (f : α → Id β) : bind x f = let y := x.run; f x := by rfl
+
+@[simp]
+theorem pure_id (x : α) : pure (f:=Id) x = x := by rfl
+
+attribute [simp] Id.run
+set_option trace.HouLean.sas.simp false
+#sas (fun (x : Float) (b? : Option Float) => (bar' x (some a) b?))
+
+#sas (fun x : Float => x + 0)
+
+#sas (fun x y : Nat => x + y)
+
+#check (fun x y : Nat => Add.add x y) rewrite_by simp
+
+
+def f2 (x y : Vector Float 3) := x[0] + y[0]
+
+set_option pp.funBinderTypes true in
+set_option trace.HouLean.sas true in
+#sas fun (x y : Vector Float 3) => f2 x y
+
+
+#sas fun (x : Option Nat) => x.getD 0
